adding syntax for natural numbers

theories/AutoSubst/PiUniv.sig
@@ -3,6 +3,12 @@ aname : Type
 term : Type
 
 tSort : sort -> term
+
 tProd : aname -> term -> (bind term in term) -> term
 tLambda : aname -> term -> (bind term in term) -> term
 tApp : term -> term -> term
+
+tNat : term
+tZero : term
+tSucc : term -> term
+tNatElim : (bind term in term) -> term -> term -> term -> term
